src/string/stringSyntax.sml
@@ -36,15 +36,19 @@ val fromHOLchar =
         Strings
  ---------------------------------------------------------------------------*)
 
-val string_ty = mk_thy_type {Tyop="string", Thy="string", Args=[]}
+val stri = inst [alpha |-> char_ty]
+
+val string_ty = mk_thy_type {Tyop="list", Thy="list", Args=[char_ty]}
 
 val implode_tm     = prim_mk_const{Name="IMPLODE",     Thy="string"}
 val explode_tm     = prim_mk_const{Name="EXPLODE",     Thy="string"}
-val emptystring_tm = prim_mk_const{Name="EMPTYSTRING", Thy="string"}
-val string_tm      = prim_mk_const{Name="STRING",      Thy="string"}
-val string_case_tm = prim_mk_const{Name="string_case", Thy="string"}
-val strlen_tm      = prim_mk_const{Name="STRLEN",      Thy="string"}
-val strcat_tm      = prim_mk_const{Name="STRCAT",      Thy="string"}
+val emptystring_tm = mk_thy_const{Name="NIL", Thy="list", Ty = string_ty}
+val string_tm      = mk_thy_const{Name="CONS", Thy="list",
+                                  Ty = char_ty --> string_ty --> string_ty}
+val string_case_tm = inst [beta |-> alpha]
+                          (stri (prim_mk_const{Name="list_case", Thy="list"}))
+val strlen_tm      = stri (prim_mk_const{Name="LENGTH",    Thy="list"})
+val strcat_tm      = stri (prim_mk_const{Name="APPEND",    Thy="list"})
 val isprefix_tm    = prim_mk_const{Name="isPREFIX",    Thy="string"};
 
 val mk_implode = C (with_exn (curry mk_comb implode_tm)) (ERR "mk_implode" "")
